Otbn/TrialDiv.v
@@ -1,0 +1,489 @@
+Require Import Coq.Init.Byte.
+Require Import Coq.Strings.String.
+Require Import Coq.micromega.Lia.
+Require Import Coq.Lists.List.
+Require Import Coq.ZArith.ZArith.
+Require Import coqutil.Map.Interface.
+Require Import coqutil.Map.OfListWord.
+Require Import coqutil.Map.Properties.
+Require Import coqutil.Map.Separation.
+Require Import coqutil.Map.SeparationLogic.
+Require Import coqutil.Semantics.OmniSmallstepCombinators.
+Require Import coqutil.Tactics.Tactics.
+Require Import coqutil.Word.Interface.
+Require Import coqutil.Word.Properties.
+Require Import coqutil.Word.LittleEndianList.
+Require Import coqutil.Z.PushPullMod.
+Require Import coqutil.Z.ZLib.
+Require Import Otbn.Model.
+Import ListNotations.
+Import Otbn.Model.Coercions.
+Local Open Scope Z_scope.
+
+(* Test out the model by trying to prove the fold_bignum function for RSA trial division. *)
+
+(***
+Original code:
+
+/**
+ * Partially reduce a value modulo m such that 2^32 mod m == 1.
+ *
+ * Returns r such that r mod m = x mod m and r < 2^35.
+ *
+ * Can be used to speed up modular reduction on certain numbers, such as 3, 5,
+ * 17, and 65537.
+ *
+ * Because we know 2^32 mod m is 1, it follows that in general 2^(32*k) for any
+ * k are all 1 modulo m. This includes 2^256, so when we receive the input as
+ * a bignum in 256-bit limbs, we can simply all the limbs together to get an
+ * equivalent number modulo m:
+ *  x = x[0] + 2^256 * x[1] + 2^512 * x[2] + ...
+ *  x \equiv x[0] + x[1] + x[2] + ... (mod F4)
+ *
+ * From there, we can essentially use the same trick to bisect the number into
+ * 128-bit, 64-bit, and 32-bit chunks and add these together to get an
+ * equivalent number modulo m. This operation is visually sort of like folding
+ * the number over itself repeatedly, which is where the function gets its
+ * name.
+ *
+ * Flags: Flags have no meaning beyond the scope of this subroutine.
+ *
+ * @param[in]  x16: dptr_x, pointer to first limb of x in dmem
+ * @param[in]  x30: plen, number of 256-bit limbs for x
+ * @param[in]  w24: constant, 2^256 - 1
+ * @param[in]  w31: all-zero
+ * @param[out] w23: r, result
+ *
+ * clobbered registers: x2, w22, w23
+ * clobbered flag groups: FG0
+ */
+fold_bignum:
+  /* Initialize constants for loop. */
+  li      x22, 22
+
+  /* Copy input pointer. */
+  addi    x2, x16, 0
+
+  /* Initialize sum to zero and clear FG0.C.
+       w23 <= 0
+       FG0.C <= 0 */
+  bn.addi  w23, w31, 0
+
+  /* Iterate through the limbs of x and add them together.
+
+     Loop invariants for iteration i (i=0..n-1):
+       x2 = dptr_x + i*32
+       x22 = 22
+       (w23 + FG0.C) \equiv x[0] + x[1] + ... + x[i-1] (mod m)
+   */
+  loop    x30, 2
+    /* Load the next limb.
+         w22 <= x[i] */
+
+    bn.lid   x22, 0(x2++)
+
+    /* Accumulate the new limb, incorporating the carry bit from the previous
+       round if there was one (this works because 2^256 \equiv 1 mod m).
+         w23 <= (w23 + x[i] + FG0.C) mod 2^256
+         FG0.C <= (w23 + x[i] + FG0.C) / 2^256 */
+    bn.addc  w23, w23, w22
+
+  /* Isolate the lower 128 bits of the sum.
+       w22 <= w23[127:0] */
+  bn.and   w22, w23, w24 >> 128
+
+  /* Add the two 128-bit halves of the sum, plus the carry from the last round
+     of the sum computation. The sum is now up to 129 bits.
+       w23 <= (w22 + (w23 >> 128) + FG0.C) */
+  bn.addc  w23, w22, w23 >> 128
+
+  /* Isolate the lower 64 bits of the sum.
+       w22 <= w23[63:0] */
+  bn.and   w22, w23, w24 >> 192
+
+  /* Add the two halves of the sum (technically 64 and 65 bits). A carry was
+     not possible in the previous addition since the value is too small. The
+     value is now up to 66 bits.
+       w23 <= (w22 + (w23 >> 64)) */
+  bn.add   w23, w22, w23 >> 64
+
+  /* Isolate the lower 32 bits of the sum.
+       w22 <= w23[31:0] */
+  bn.and   w22, w23, w24 >> 224
+
+  /* Add the two halves of the sum (technically 32 and 34 bits). A carry was
+     not possible in the previous addition since the value is too small.
+       w23 <= (w22 + (w23 >> 32)) */
+  bn.add   w23, w22, w23 >> 32
+
+  ret
+
+ ***)
+
+(* generic bignums *)
+Section WithWord.
+  Context {width} {word : word.word width} {word_ok : word.ok word}.
+
+  Definition eval (x : list word) : Z :=
+    fold_right (fun xi acc => word.unsigned xi + 2^width*acc) 0 x.
+
+  Lemma eval_nil : eval [] = 0.
+  Proof. reflexivity. Qed.
+
+  Lemma eval_cons x0 x : eval (x0 :: x) = word.unsigned x0 + 2^width*(eval x).
+  Proof. reflexivity. Qed.
+
+  Lemma eval_app x y n :
+    Z.of_nat (length x) = n ->
+    eval (x ++ y) = eval x + 2^(width*n) * (eval y).
+  Proof.
+    intros; subst. generalize dependent y.
+    induction x; intros; [ rewrite !app_nil_l, Z.mul_0_r, eval_nil; lia | ].
+    pose proof word.width_pos.
+    rewrite <-app_comm_cons, !eval_cons, IHx.
+    cbn [length]. rewrite Nat2Z.inj_succ, Z.mul_succ_r.
+    rewrite Z.pow_add_r; lia.
+  Qed.
+
+  Lemma eval_bounds x :
+    0 <= eval x < 2^(width*Z.of_nat (length x)).
+  Proof.
+    induction x as [|x0 ?]; intros; cbn [length]; [ rewrite eval_nil; lia | ].
+    pose proof word.unsigned_range x0. pose proof word.width_pos.
+    rewrite eval_cons. rewrite Nat2Z.inj_succ, Z.mul_succ_r, Z.pow_add_r by lia.
+    nia.
+  Qed.
+End WithWord.
+
+Section __.
+  Context {word32 : word.word 32} {word32_ok : word.ok word32}.
+  Context {word256 : word.word 256} {word256_ok : word.ok word256}.
+  Context {regfile : map.map reg word32} {regfile_ok : map.ok regfile}.
+  Context {wregfile : map.map wreg word256} {wregfile_ok : map.ok wregfile}.
+  Context {flagfile : map.map flag bool} {flagfile_ok : map.ok flagfile}.
+  Context {mem : map.map word32 byte} {mem_ok : map.ok mem}.
+  Add Ring wring32: (@word.ring_theory 32 word32 word32_ok).
+  Add Ring wring256: (@word.ring_theory 256 word256 word256_ok).
+
+  Definition fold_bignum : otbn_function :=
+    ("fold_bignum"%string,
+      map.empty,
+      [(Addi x22 x0 22 : insn);
+       (Addi x2 x16 0 : insn);
+       (Bn_addi w23 w31 0 FG0 : insn);
+       (Loop x30 : insn);
+       (Bn_lid x22 false x2 true 0 : insn);
+       (Bn_addc w23 w23 w22 0 FG0 : insn);
+       (LoopEnd : insn);
+       (Bn_and w22 w23 w24 (-128) FG0 : insn);
+       (Bn_addc w23 w22 w23 (-128) FG0 : insn);
+       (Bn_and w22 w23 w24 (-192) FG0 : insn);
+       (Bn_add w23 w22 w23 (-64) FG0 : insn);
+       (Bn_and w22 w23 w24 (-224) FG0 : insn);
+       (Bn_add w23 w22 w23 (-32) FG0 : insn);
+       (Ret : insn)]).
+
+  Definition fold_bignum_spec (x : list word256) (n : nat) : Z :=
+    let x := fold_left Z.add (map word.unsigned x) 0 in
+    let x := x mod 2^128 + x / 2^128 in
+    let x := x mod 2^64 + x / 2^64 in
+    let x := x mod 2^32 + x / 2^32 in
+    x.
+
+  Lemma fold_bignum_step x y m :
+    y mod m = 1 -> 0 < m -> 0 < y ->
+    (x mod y + x / y) mod m = x mod m.
+  Proof.
+    intros. rewrite (Z.mod_eq x y) by lia.
+    Z.push_mod. replace (y mod m) with 1 by lia.
+    rewrite Z.mul_1_l. Z.push_pull_mod.
+    f_equal; lia.
+  Qed.
+
+  Lemma fold_left_add_init a x : fold_left Z.add x a = a + fold_left Z.add x 0.
+  Proof.
+    generalize dependent a. induction x; intros; [ cbn [fold_left]; lia | ].
+    cbn [fold_left]. rewrite !IHx with (a:=_ + _).
+    lia.
+  Qed.
+
+  Lemma fold_bignum_array_correct m (x : list word256) :
+    2^256 mod m = 1 -> 0 < m ->
+    (fold_left Z.add (map word.unsigned x) 0) mod m = (eval x) mod m.
+  Proof.
+    intros; induction x; intros; [ reflexivity | ].
+    cbn [map fold_left]. rewrite Z.add_0_l, eval_cons.
+    rewrite fold_left_add_init. Z.push_mod.
+    rewrite IHx. replace (2^256 mod m) with 1 by lia.
+    rewrite Z.mul_1_l. Z.push_pull_mod. f_equal; lia.
+  Qed.
+
+  Definition bignum_at (ptr : word32) (v : list word256) : mem -> Prop :=
+    bytes_at ptr (le_split (Z.to_nat 32 * length v) (eval v)).
+
+  Lemma split_bignum_nth n ptr v :
+    (n < length v)%nat ->
+    Lift1Prop.iff1 (bignum_at ptr v)
+      (Lift1Prop.ex1
+         (fun v0 =>
+            Lift1Prop.ex1
+              (fun vn =>
+                 Lift1Prop.ex1
+                   (fun v1 =>
+                      (emp (length v0 = n)
+                       * emp (v = v0 ++ [vn] ++ v1)
+                       * bignum_at ptr v0
+                       * word_at (word.add ptr (word.of_Z (32*Z.of_nat n))) vn
+                       * bignum_at ptr v1)%sep)))).
+  Admitted.
+
+  (* helper lemma that makes it easier to prove the folding steps *)
+  Lemma pow2_mod1_multiple w i m :
+    0 <= w ->
+    0 <= i ->
+    1 < m ->
+    2^w mod m = 1 ->
+    2^(w*i) mod m = 1.
+  Proof.
+    intros. generalize dependent w. generalize dependent i.
+    (* natlike induction on i *)
+    lazymatch goal with
+    | |- forall i, 0 <= i -> ?P =>
+        apply (natlike_ind (fun i => P))
+    end.
+    { intros. rewrite Z.mul_0_r, Z.pow_0_r, Z.mod_1_l by lia. lia. }
+    { intros. rewrite Z.mul_succ_r, Z.pow_add_r by lia. Z.push_mod.
+      repeat match goal with H : context [2^_ mod m = 1] |- _ => rewrite H by lia end.
+      rewrite Z.mul_1_r, Z.mod_1_l by lia; lia. }
+  Qed.
+
+  (* TODO: move *)
+  Lemma carry_bit_addc_div x y c :
+    0 <= x < 2^256 ->
+    0 <= y < 2^256 ->
+    Z.b2z (carry_bit (x + y + Z.b2z c)) = (x + y + Z.b2z c) / 2^256.
+  Admitted.
+
+  Lemma fold_bignum_correct :
+    forall regs wregs flags dmem cstack lstack
+           (dptr_x plen : word32) x m R,
+      (length lstack < 8)%nat ->
+      is_word_aligned 32 dptr_x = true ->
+      word.unsigned dptr_x + 32 * word.unsigned plen < DMEM_BYTES ->
+      map.get regs (gpreg x16) = Some dptr_x ->
+      map.get regs (gpreg x30) = Some plen ->
+      map.get wregs (wdreg w24) = Some (word.of_Z (2^256 - 1)) ->
+      map.get wregs (wdreg w31) = Some (word.of_Z 0) ->
+      0 <= eval x <= 2^(256*word.unsigned plen) ->
+      (2^32 mod m = 1) ->
+      1 < m ->
+      word.unsigned plen = Z.of_nat (length x) ->
+      (* TODO: probably 0 < length x is enough here with a bit more
+         proof effort, but it's not clearly necessary *)
+      (1 < length x)%nat ->
+      (bignum_at dptr_x x * R)%sep dmem ->
+      returns
+        (fetch:=fetch_ctx [fold_bignum])
+        "fold_bignum"%string regs wregs flags dmem cstack lstack
+        (fun regs' wregs' flags' dmem' =>           
+           dmem = dmem'
+           /\ (exists v,
+                  map.get wregs' (wdreg w23) = Some v
+                  /\ word.unsigned v mod m = eval x mod m
+                  /\ 0 <= word.unsigned v < 2^33)
+           /\ clobbers [flagM FG0; flagL FG0; flagZ FG0; flagC FG0] flags flags'
+           /\ clobbers [wdreg w22; wdreg w23] wregs wregs'
+           /\ clobbers [gpreg x2] regs regs').
+  Proof.    
+    cbv [fold_bignum returns]. intros; subst.
+    track_registers_init.
+
+    (* helpful assertions *)
+    assert (2^256 mod m = 1) by (apply (pow2_mod1_multiple 32 8); lia).
+    assert (2^128 mod m = 1) by (apply (pow2_mod1_multiple 32 4); lia).
+    assert (2^64 mod m = 1) by (apply (pow2_mod1_multiple 32 2); lia).
+
+    straightline_step.
+    straightline_step.
+    straightline_step.
+
+    (*
+     Loop invariants (at end of loop) for iteration i (i=n..1):
+       x2 = dptr_x + (n-i+1)*32
+       x22 = 22
+       (w23 + FG0.C) \equiv x[0] + x[1] + ... + x[n-i] (mod m)
+     *)
+    (* loop; use loop invariant lemma *)
+    let regs := lazymatch goal with
+                  |- eventually run1 _ (otbn_busy  _ ?regs ?wregs ?flags ?dmem _ _) =>
+                    regs end in
+    let wregs := lazymatch goal with
+                  |- eventually run1 _ (otbn_busy  _ ?regs ?wregs ?flags ?dmem _ _) =>
+                    wregs end in
+    let flags := lazymatch goal with
+                  |- eventually run1 _ (otbn_busy  _ ?regs ?wregs ?flags ?dmem _ _) =>
+                    flags end in
+    let dmem := lazymatch goal with
+                  |- eventually run1 _ (otbn_busy  _ ?regs ?wregs ?flags ?dmem _ _) =>
+                    dmem end in
+    let loop_end_pc := find_loop_end in
+    eapply loop_invariant
+      with
+      (end_pc:=loop_end_pc)
+      (invariant :=
+         fun i regs' wregs' flags' dmem' =>
+           map.get regs' (gpreg x2) = Some (word.add dptr_x
+                                              (word.of_Z (32*(Z.of_nat (length x - i)))))
+           /\ map.get regs' (gpreg x22) = Some (addi_spec (word.of_Z 0) 22)
+           /\ (exists acc c,
+                  map.get wregs' (wdreg w23) = Some acc
+                  /\ map.get flags' (flagC FG0) = Some c
+                  /\ (word.unsigned acc + Z.b2z c) mod m
+                     = eval (List.firstn (length x - i) x) mod m)
+           /\ dmem' = dmem
+           /\ clobbers [flagM FG0; flagL FG0; flagZ FG0; flagC FG0] flags flags'
+           /\ clobbers [wdreg w22; wdreg w23] wregs wregs'
+           /\ clobbers [gpreg x2; gpreg x22] regs regs').
+    { reflexivity. }
+    { reflexivity. }
+    { simplify_side_condition; reflexivity. }
+    { apply Z2Nat.id; lia. }
+    { lia. }
+    { lia. }
+    { (* prove invariant holds at start *)
+      ssplit; simplify_side_condition; zsimplify; try reflexivity.
+      all:try replace (Z.to_nat (word.unsigned plen)) with (length x) by lia.
+      all:rewrite ?Nat.sub_diag.
+      all:try solve [apply map.only_differ_same].
+      { (* memory pointer *)
+        subst_lets. apply f_equal.
+        cbv [addi_spec]. destruct_one_match; try lia; [ ].
+        apply f_equal. apply f_equal. ring. }
+      { (* accumulator equation *)
+        rewrite @eval_nil. subst_lets.
+        rewrite word.unsigned_of_Z_0.
+        reflexivity. } }
+    { (* invariant step; proceed through loop and prove invariant still holds *)
+      intros.
+      repeat lazymatch goal with
+             | H : _ /\ _ |- _ => destruct H
+             | H : exists _, _ |- _ => destruct H
+             | _ => progress subst
+             end.
+
+      (* assert that the pointer is in bounds of DMEM *)
+      lazymatch goal with
+      | H : map.get ?regs (gpreg _) = Some (word.add dptr_x ?offset) |- context [?regs] =>
+          assert (word.unsigned (word.add dptr_x offset) + 32 < DMEM_BYTES)
+      end.
+      { rewrite word.unsigned_add.
+        pose proof word.unsigned_range dptr_x.
+        assert (DMEM_BYTES < 2^32) by (vm_compute; congruence).
+        rewrite word.unsigned_of_Z_nowrap by lia.
+        cbv [word.wrap]; rewrite Z.mod_small by lia. lia. }
+
+      (* rewrite the seplogic statement to expose the word we're going to load *)
+      lazymatch goal with
+      | H : sep (bignum_at _ _) _ ?m |- context[?m] =>
+          seprewrite_in (split_bignum_nth (length x - S i)) H; [ lia .. | ]
+      end.
+      extract_ex1_and_emp_in_hyps.
+      subst.
+
+      straightline_step.
+      straightline_step.
+      
+      (* end of loop; use loop-end helper lemma *)
+      eapply eventually_loop_end; [ reflexivity .. | ].
+      destruct_one_match.
+      { (* case: i = 0, loop ends *)
+        intros; subst. eapply eventually_done.
+        left. do 4 eexists; ssplit; [ .. | reflexivity ]; solve_map; [ | ].
+        { simplify_side_condition; subst_lets; zsimplify.
+          apply (f_equal Some). apply word.unsigned_inj.
+          rewrite !word.unsigned_add, !word.unsigned_of_Z.
+          cbv [word.wrap]. Z.push_pull_mod. f_equal. lia. }
+        { do 2 eexists; subst_lets; ssplit; try reflexivity; [ ].
+          (* at this point the remainder of the bignum is nil *)
+          lazymatch goal with
+          | |- context[?x ++ [?y] ++ ?z] =>
+              destruct z;
+              [ rewrite !app_nil_r in *
+              | rewrite ?app_length in *; cbn [length] in *; lia ]
+          end.
+          rewrite Nat.sub_0_r, List.firstn_all.
+          erewrite !eval_app, eval_cons, eval_nil by eauto.
+          rewrite Z.add_0_r.
+          lazymatch goal with
+          | H : _ = eval (List.firstn (length (?a ++ [?b]) - 1) (?a ++ [?b])) mod m |- _ =>
+              rewrite List.firstn_app_l in H by (rewrite app_length; cbn [length]; lia)
+          end.
+          rewrite carry_bit_addc_div by (eauto using word.unsigned_range).
+          rewrite !word.unsigned_add, !word.unsigned_of_Z by lia.
+          cbv [word.wrap]. Z.push_pull_mod.
+          (* for some reason the mod m doesn't get fully pulled out *)
+          rewrite <-Z.add_mod by lia.
+          rewrite fold_bignum_step by lia.
+          Z.push_mod. rewrite pow2_mod1_multiple by lia.
+          lazymatch goal with H : _ = eval ?v mod m |- _ => rewrite <-H end.
+          rewrite Z.mul_1_l. Z.push_pull_mod.
+          f_equal; lia. } }
+      { (* case: 0 < i, loop continues *)
+        intros; subst. eapply eventually_done.
+        (* prove that the remaining length of the bignum matches the remaining iterations *)
+        lazymatch goal with
+        | H : (?i < Z.to_nat (word.unsigned plen))%nat |- context[?x ++ [?y] ++ ?z] =>
+            assert (i = length z)%nat
+            by (rewrite ?app_length in *; cbn [length] in *; destruct x, z; cbn [length] in *;
+                lia)
+        end.
+        left. do 4 eexists; ssplit; [ .. | reflexivity ]; solve_map; [ | ].
+        { simplify_side_condition; subst_lets; zsimplify.
+          apply (f_equal Some). apply word.unsigned_inj.
+          rewrite !word.unsigned_add, !word.unsigned_of_Z.
+          cbv [word.wrap]. Z.push_pull_mod. f_equal. lia. }
+        { do 2 eexists. ssplit; eauto; [ ]. subst_lets.
+          lazymatch goal with
+          | H : _ = eval (List.firstn (length (?a ++ [?b] ++ ?c) - _) (?a ++ [?b] ++ ?c)) mod m
+            |- _ =>
+              rewrite List.firstn_app_l in H by (rewrite ?app_length; cbn [length]; lia)
+          end.
+          rewrite app_assoc.
+          rewrite List.firstn_app_l by (rewrite ?app_length; cbn [length]; lia).
+          erewrite eval_app, eval_cons, eval_nil by reflexivity.
+          rewrite carry_bit_addc_div by (eauto using word.unsigned_range).
+          rewrite !word.unsigned_add, !word.unsigned_of_Z by lia.
+          cbv [word.wrap]. Z.push_pull_mod.
+          (* for some reason the mod m doesn't get fully pulled out *)
+          rewrite <-Z.add_mod by lia.
+          rewrite fold_bignum_step by lia.
+          zsimplify. Z.push_mod. rewrite pow2_mod1_multiple by lia.
+          lazymatch goal with H : _ = eval ?v mod m |- _ => rewrite <-H end.
+          zsimplify. f_equal; lia. } } }
+
+    
+    (* invariant implies postcondition (i.e. post-loop code) *)
+    rewrite Nat.sub_0_r. intros.
+    repeat lazymatch goal with
+           | H : exists _, _ |- _ => destruct H
+           | H : _ /\ _ |- _ => destruct H
+           | H : Some _ = Some _ |- _ => inversion H; clear H; subst
+           | _ => progress subst
+           end.
+    simplify_side_condition.
+
+    track_registers_combine.
+
+    print_next_insn.
+    Print
+      straightline_step.
+    eapply eventually_step_cps; simplify_side_condition.
+
+    
+    
+    intros; subst. eapply eventually_ret; [ reflexivity | eassumption | ].
+    ssplit; eauto.
+    print_next_insn.
+    (* end of loop *)
+
+  Qed.
